<?xml version="1.0" encoding="UTF-8"?>
<!-- 
    WARNING:  THIS IS A WORKING DRAFT ONTOLOGY AND STILL UNDER DEVELOPMENT, this file will change frequently and significantly as development continues.
    
    Note:  http://audio.biblioteko-o.org/ is a placeholder (fake) namespace for the LD4P/L Measurements ontology extension until a proper home is found
  -->


<rdf:RDF xmlns="http://audio.biblioteko-o.org/"
    xmlns:bf="http://id.loc.gov/ontologies/bibframe/" xmlns:bib="http://bibliotek-o.org/ontology/"
    xmlns:dcterms="http://purl.org/dc/terms/" xmlns:owl="http://www.w3.org/2002/07/owl#"
    xmlns:rdf="http://www.w3.org/1999/02/22-rdf-syntax-ns#"
    xmlns:rdfs="http://www.w3.org/2000/01/rdf-schema#"
    xmlns:skos="http://www.w3.org/2004/02/skos/core#" xmlns:xsd="http://www.w3.org/2001/XMLSchema#"
    xmlns:foaf="http://xmlns.com/foaf/0.1#" xmlns:vann="http://purl.org/vocab/vann/"
    xmlns:voaf="http://purl.org/vocommons/voaf#">

<!-- ONTOLOGY DECLARATION -->

    <owl:Ontology rdf:about="http://audio.biblioteko-o.org/">
        <owl:versionInfo rdf:datatype="http://www.w3.org/2001/XMLSchema#string">Version
            0.0</owl:versionInfo>
        <rdfs:label xml:lang="en">Audio extension of bibliotek-o</rdfs:label>
        <vann:preferredNamespacePrefix>audio</vann:preferredNamespacePrefix>
        <rdfs:comment xml:lang="en">This measurements ontology was developed as a stand alone
            ontology as part of the bibliotek-o BIBFRAME 2.0 extension ontology
            project</rdfs:comment>
        <voaf:extends rdf:resource="http://bibliotek-o.org/ontology/"/>
        <voaf:specializes rdf:resource="http://bibliotek-o.org/ontology/"/>
        <voaf:extends rdf:resource="http://id.loc.gov/ontologies/bibframe/"/>
        <voaf:specializes rdf:resource="http://id.loc.gov/ontologies/bibframe/"/>
    </owl:Ontology>


    <!-- CLASSES -->
    
<owl:Class rdf:about="http://audio.biblioteko-o.org/CaptureAndStorageTechnique">
    <rdfs:label>Capture and storage technique</rdfs:label>
    <skos:definition>The type of equipment used in making the recording, as opposed to the type of equipment required for playback.</skos:definition>
    <skos:scopeNote xml:lang="en">This class is derived from the MARC 21 007 position 13 for sound recordings, https://www.loc.gov/marc/bibliographic/bd007s.html..</skos:scopeNote>
</owl:Class>
    
<owl:Class rdf:about="http://audio.biblioteko-o.org/CuePointMarkerNote">
    <rdfs:label>Cue point markers</rdfs:label>
    <rdfs:subClassOf rdf:resource="http://id.loc.gov/ontologies/bibframe/Note"/>
    <skos:definition>A note explaining that there are Cue point markers on the disc. (about the same as beat markers) Wording: Cue point markers on disc[s].</skos:definition>
</owl:Class>
    
<owl:Class rdf:about="http://audio.biblioteko-o.org/NumberedSRJacketNote">
    <rdfs:label>Numbered SR Jacket Note</rdfs:label>
    <rdfs:subClassOf rdf:resource="http://audio.biblioteko-o.org/WritingOnAlbumNote"/>
    <skos:definition>A note explaining this copy was numbered by Bambaataa on the jacket. Wording: Numbered #[x] on jacket. </skos:definition>
</owl:Class>
    
<owl:Class rdf:about="http://audio.biblioteko-o.org/InitialsOrNumberOnLabelNote">
    <rdfs:label>Initials and/or numbers on disc label</rdfs:label>
    <rdfs:subClassOf rdf:resource="http://audio.biblioteko-o.org/WritingOnAlbumNote"/>
    <skos:definition>A note explaining this copy was numbered and/or initialed by Bambaataa on the label. Wording: Numbered #[x] on disc label. </skos:definition>
</owl:Class>
    
<owl:Class rdf:about="http://audio.biblioteko-o.org/NotInOriginalJacketNote">
    <rdfs:label>SR doesn’t match the jacket.</rdfs:label>
    <rdfs:subClassOf rdf:resource="http://id.loc.gov/ontologies/bibframe/Note"/>
    <skos:definition>A note explaining SR doesn’t match the jacket. Wording: Not in original jacket. </skos:definition>
</owl:Class>

<owl:Class rdf:about="http://audio.biblioteko-o.org/PerformedMusic">
    <rdfs:label>Performed Music</rdfs:label>
    <rdfs:subClassOf rdf:resource="http://id.loc.gov/ontologies/bibframe/Audio"/>
    <skos:definition>An audio work consisting of content expressed through music in an audible form, not necessarily performed live. To denote a live performance a bib:PerformedMusic should be linked to a live event.</skos:definition>
    <skos:scopeNote xml:lang="en">This class is derived from the RDA Content Type: http://rdaregistry.info/termList/RDAContentType/1011.</skos:scopeNote>
</owl:Class>
    
<owl:Class rdf:about="http://audio.biblioteko-o.org/PostItNoteNote">
    <rdfs:label>Post-It Note on LP</rdfs:label>
    <rdfs:subClassOf rdf:resource="http://id.loc.gov/ontologies/bibframe/Note"/>
    <skos:definition>A note explaining there is a post-it on the LP jacket, Wording: Sticky note attached to jacket, reading: “[text]” (most likely from the first round of sorting done in New York City). </skos:definition>
</owl:Class>
    
<owl:Class rdf:about="http://audio.biblioteko-o.org/SignatureNote">
    <rdfs:label>Signature Note</rdfs:label>
    <rdfs:subClassOf rdf:resource="http://audio.biblioteko-o.org/WritingOnAlbumNote"/>
    <skos:definition>A note explaining there is a signature on the copy, Wording: Provenance: Afrika Bambaataa (signature). Or if signed with initials: Provenance: A[frika] B[ambaataa] (signature). </skos:definition>
</owl:Class>
  
<owl:Class rdf:about="http://audio.biblioteko-o.org/Sounds">
    <rdfs:label>Sounds</rdfs:label>
    <rdfs:subClassOf rdf:resource="http://id.loc.gov/ontologies/bibframe/Audio"/>
    <skos:definition>An audio work consisting of content other than language or music, expressed in an audible form.</skos:definition>
    <skos:scopeNote xml:lang="en">This class is derived from the RDA Content Type: http://rdaregistry.info/termList/RDAContentType/1012.</skos:scopeNote>
</owl:Class>
  
<owl:Class rdf:about="http://audio.biblioteko-o.org/SpokenWord">
    <rdfs:label>Spoken word</rdfs:label>
    <rdfs:subClassOf rdf:resource="http://id.loc.gov/ontologies/bibframe/Audio"/>
    <skos:definition>An audio work consisting of content expressed through language in an audible form.</skos:definition>
    <skos:scopeNote xml:lang="en">This class is derived from the RDA Content Type: http://rdaregistry.info/termList/RDAContentType/1013.</skos:scopeNote>
</owl:Class>
    
<owl:Class rdf:about="http://audio.biblioteko-o.org/TapeOnLPDiscLabelOrCoverNote">
    <rdfs:label>Tape on LP’s disc label or cover</rdfs:label>
    <rdfs:subClassOf rdf:resource="http://id.loc.gov/ontologies/bibframe/Note"/>
    <skos:definition>A note explaining there is tape on disc label or cover to obscure the title, artist, etc. (Bam put this tape on LPs) Wording: Title [or artist’s name, etc.] obscured with black tape [or white sticker] on label [or jacket].</skos:definition>
</owl:Class>
    
<owl:Class rdf:about="http://audio.biblioteko-o.org/TracksOfInterestNote">
    <rdfs:label>Track numbers of interest indicated</rdfs:label>
    <rdfs:subClassOf rdf:resource="http://audio.biblioteko-o.org/WritingOnAlbumNote"/>
    <skos:definition>A note explaining there tracks marked with a star, or track numbers of interest listed. Wording: Track numbers of interest indicated on jacket [or label]. </skos:definition>
</owl:Class>  

<owl:Class rdf:about="http://audio.biblioteko-o.org/TwoCopiesInSameSleeveNote">
    <rdfs:label>Two copies housed together</rdfs:label>
    <rdfs:subClassOf rdf:resource="http://id.loc.gov/ontologies/bibframe/Note"/>
    <skos:definition>A note explaining there are two copies of the same LP in the same sleeve. Wording: Two copies housed together.</skos:definition>
</owl:Class>
    
<owl:Class rdf:about="http://audio.biblioteko-o.org/WritingOnAlbumNote">
    <rdfs:label>Writing directly on the album cover, etc.</rdfs:label>
    <rdfs:subClassOf rdf:resource="http://id.loc.gov/ontologies/bibframe/Note"/>
    <skos:definition>A note explaining there is writing directly on the LP jacket, sleeve, label, etc. This was done by Bambaataa, Wording: Manuscript note on outer jacket [etc.]:  “[text].” </skos:definition>
</owl:Class>

  
    <!-- OBJECT PROPERTIES -->
    
    <!-- Individuals -->
    
    
    <owl:NamedIndividual rdf:about="http://audio.biblioteko-o.org/acousticalCaptureDirectStorage">
        <rdf:type rdf:resource="http://audio.biblioteko-o.org/CaptureAndStorageTechnique"/>
        <rdfs:label xml:lang="en">Acoustical capture, direct storage</rdfs:label>
    </owl:NamedIndividual>
    
    <owl:NamedIndividual rdf:about="http://audio.biblioteko-o.org/DirectStorageNotAcoustical">
        <rdf:type rdf:resource="http://audio.biblioteko-o.org/CaptureAndStorageTechnique"/>
        <rdfs:label xml:lang="en">Direct storage, not acoustical</rdfs:label>
    </owl:NamedIndividual>
    
    <owl:NamedIndividual rdf:about="http://audio.biblioteko-o.org/DirectStorage">
        <rdf:type rdf:resource="http://audio.biblioteko-o.org/CaptureAndStorageTechnique"/>
        <rdfs:label xml:lang="en">Direct storage</rdfs:label>
    </owl:NamedIndividual>
    
    <owl:NamedIndividual rdf:about="http://audio.biblioteko-o.org/AnalogElectricalStorage">
        <rdf:type rdf:resource="http://audio.biblioteko-o.org/CaptureAndStorageTechnique"/>
        <rdfs:label xml:lang="en">Analog electrical storage</rdfs:label>
    </owl:NamedIndividual>
    
</rdf:RDF>